src/SDK/Keyring/AwsKms/AwsKmsMrkAwareSymmetricKeyring.dfy
@@ -1,0 +1,548 @@
+// Copyright Amazon.com Inc. or its affiliates. All Rights Reserved.
+// SPDX-License-Identifier: Apache-2.0
+
+include "../Defs.dfy"
+include "../../Materials.dfy"
+include "../../AlgorithmSuite.dfy"
+include "../../../StandardLibrary/StandardLibrary.dfy"
+include "../../../KMS/KMSUtils.dfy"
+include "../../../KMS/AmazonKeyManagementService.dfy"
+include "../../../KMS/AwsKmsArnParsing.dfy"
+include "../../../Util/UTF8.dfy"
+include "../../../../libraries/src/Collections/Sequences/Seq.dfy"
+include "../../../../libraries/src/Collections/Sequences/Closures.dfy"
+include "../../Serializable.dfy"
+include "Constants.dfy"
+include "AwsKmsMrkMatchForDecrypt.dfy"
+
+module {:extern "AwsKmsMrkAwareSymmetricKeyring"} AwsKmsMrkAwareSymmetricKeyring {
+  import opened StandardLibrary
+  import opened Wrappers
+  import opened UInt = StandardLibrary.UInt
+  import opened AwsKmsArnParsing
+  import opened AmazonKeyManagementService
+  import opened Seq
+  import opened Closures
+  import opened Constants
+  import opened AwsKmsMrkMatchForDecrypt
+  import Serializable
+  import AlgorithmSuite
+  import opened KeyringDefs
+  import Materials
+  import opened KMSUtils
+  import UTF8
+
+  //= compliance/framework/aws-kms/aws-kms-mrk-aware-symmetric-keyring.txt#2.5
+  //= type=implication
+  //# MUST implement the AWS Encryption SDK Keyring interface (../keyring-
+  //# interface.md#interface)
+  class AwsKmsMrkAwareSymmetricKeyring
+    extends Keyring
+  {
+
+    const client: IAmazonKeyManagementService
+    const awsKmsKey: AwsKmsIdentifierString
+    const awsKmsArn: AwsKmsIdentifier
+    const grantTokens: KMSUtils.GrantTokens
+
+    constructor (
+      //= compliance/framework/aws-kms/aws-kms-mrk-aware-symmetric-keyring.txt#2.6
+      //= type=implication
+      //# The AWS KMS SDK client MUST NOT be null.
+      client: IAmazonKeyManagementService,
+      awsKmsKey: string,
+      grantTokens: seq<KMSUtils.GrantToken>
+    )
+      //= compliance/framework/aws-kms/aws-kms-mrk-aware-symmetric-keyring.txt#2.6
+      //= type=implication
+      //# The AWS KMS key identifier MUST NOT be null or empty.
+      //# The AWS KMS
+      //# key identifier MUST be a valid identifier (aws-kms-key-arn.md#a-
+      //# valid-aws-kms-identifier).
+      requires ParseAwsKmsIdentifier(awsKmsKey).Success?
+      requires UTF8.IsASCIIString(awsKmsKey)
+      requires 0 < |awsKmsKey| <= MAX_AWS_KMS_IDENTIFIER_LENGTH
+      requires 0 <= |grantTokens| <= KMSUtils.MAX_GRANT_TOKENS
+    {
+      var awsKmsArn    := ParseAwsKmsIdentifier(awsKmsKey);
+      this.client      := client;
+      this.awsKmsKey   := awsKmsKey;
+      this.awsKmsArn   := awsKmsArn.value;
+      this.grantTokens := grantTokens;
+    }
+
+    predicate Valid()
+      reads this, Repr
+      ensures Valid() ==> this in Repr
+    {
+      && this in Repr
+    }
+
+    //= compliance/framework/aws-kms/aws-kms-mrk-aware-symmetric-keyring.txt#2.7
+    //= type=implication
+    //# OnEncrypt MUST take encryption materials (structures.md#encryption-
+    //# materials) as input.
+    method OnEncrypt(materials: Materials.ValidEncryptionMaterials)
+      returns (res: Result<Materials.ValidEncryptionMaterials, string>)
+      requires Valid()
+      ensures Valid()
+      ensures OnEncryptPure(materials, res)
+      //= compliance/framework/aws-kms/aws-kms-mrk-aware-symmetric-keyring.txt#2.7
+      //= type=implication
+      //# If the input encryption materials (structures.md#encryption-
+      //# materials) do not contain a plaintext data key OnEncrypt MUST attempt
+      //# to generate a new plaintext data key by calling AWS KMS
+      //# GenerateDataKey (https://docs.aws.amazon.com/kms/latest/APIReference/
+      //# API_GenerateDataKey.html).
+      ensures
+        && materials.plaintextDataKey.None?
+      ==>
+        GenerateDataKeyCalledWith(
+          //= compliance/framework/aws-kms/aws-kms-mrk-aware-symmetric-keyring.txt#2.7
+          //= type=implication
+          //# If the keyring calls AWS KMS GenerateDataKeys, it MUST use the
+          //# configured AWS KMS client to make the call.
+          this.client,
+          //= compliance/framework/aws-kms/aws-kms-mrk-aware-symmetric-keyring.txt#2.7
+          //= type=implication
+          //# The keyring MUST call
+          //# AWS KMS GenerateDataKeys with a request constructed as follows:
+          GenerateDataKeyRequest(
+            materials.encryptionContext,
+            this.grantTokens,
+            this.awsKmsKey,
+            materials.algorithmSuiteID.KDFInputKeyLength() as int32
+          ))
+
+      //= compliance/framework/aws-kms/aws-kms-mrk-aware-symmetric-keyring.txt#2.7
+      //= type=implication
+      //# *  OnEncrypt MUST output the modified encryption materials
+      //# (structures.md#encryption-materials)
+      ensures 
+        && materials.plaintextDataKey.None?
+        && res.Success?
+      ==>
+        && res.value.plaintextDataKey.Some?
+        && |res.value.encryptedDataKeys| == |materials.encryptedDataKeys| + 1
+        //= compliance/framework/aws-kms/aws-kms-mrk-aware-symmetric-keyring.txt#2.7
+        //= type=implication
+        //# If the Generate Data Key call succeeds, OnEncrypt MUST verify that
+        //# the response "Plaintext" length matches the specification of the
+        //# algorithm suite (algorithm-suites.md)'s Key Derivation Input Length
+        //# field.
+        && materials.algorithmSuiteID.ValidPlaintextDataKey(res.value.plaintextDataKey.value)
+        //= compliance/framework/aws-kms/aws-kms-mrk-aware-symmetric-keyring.txt#2.7
+        //= type=implication
+        //# If verified, OnEncrypt MUST do the following with the response
+        //# from AWS KMS GenerateDataKey
+        //# (https://docs.aws.amazon.com/kms/latest/APIReference/
+        //# API_GenerateDataKey.html):
+        && GenerateDataKeyResult(
+            Last(res.value.encryptedDataKeys).ciphertext,
+            res.value.plaintextDataKey.value
+          )
+
+      //= compliance/framework/aws-kms/aws-kms-mrk-aware-symmetric-keyring.txt#2.7
+      //= type=implication
+      //# Given a plaintext data key in the encryption materials
+      //# (structures.md#encryption-materials), OnEncrypt MUST attempt to
+      //# encrypt the plaintext data key using the configured AWS KMS key
+      //# identifier.
+      ensures 
+        && materials.plaintextDataKey.Some?
+      ==>
+        && EncryptCalledWith(
+          //= compliance/framework/aws-kms/aws-kms-mrk-aware-symmetric-keyring.txt#2.7
+          //= type=implication
+          //# The keyring MUST call AWS KMS Encrypt
+          //# (https://docs.aws.amazon.com/kms/latest/APIReference/
+          //# API_Encrypt.html) using the configured AWS KMS client.
+          this.client,
+          //= compliance/framework/aws-kms/aws-kms-mrk-aware-symmetric-keyring.txt#2.7
+          //= type=implication
+          //# The keyring
+          //# MUST AWS KMS Encrypt call with a request constructed as follows:
+          EncryptRequest(
+            materials.encryptionContext,
+            this.grantTokens,
+            this.awsKmsKey,
+            materials.plaintextDataKey.value
+          ))
+
+      //= compliance/framework/aws-kms/aws-kms-mrk-aware-symmetric-keyring.txt#2.7
+      //= type=implication
+      //# If all Encrypt calls succeed, OnEncrypt MUST output the modified
+      //# encryption materials (structures.md#encryption-materials).
+      ensures 
+        && materials.plaintextDataKey.Some?
+        && res.Success?
+      ==>
+        //= compliance/framework/aws-kms/aws-kms-mrk-aware-symmetric-keyring.txt#2.7
+        //= type=implication
+        //# If verified, OnEncrypt MUST do the following with the
+        //# response from AWS KMS Encrypt
+        //# (https://docs.aws.amazon.com/kms/latest/APIReference/
+        //# API_Encrypt.html):
+        && |res.value.encryptedDataKeys| == |materials.encryptedDataKeys| + 1
+        && EncryptResult(Last(res.value.encryptedDataKeys).ciphertext)
+    {
+      if materials.plaintextDataKey.None? {
+        var generatorRequest := GenerateDataKeyRequest(
+          materials.encryptionContext,
+          this.grantTokens,
+          this.awsKmsKey,
+          materials.algorithmSuiteID.KDFInputKeyLength() as int32
+        );
+
+        var maybeGenerateResponse := GenerateDataKey(this.client, generatorRequest);
+
+        //= compliance/framework/aws-kms/aws-kms-mrk-aware-symmetric-keyring.txt#2.7
+        //# If the call to AWS KMS GenerateDataKey
+        //# (https://docs.aws.amazon.com/kms/latest/APIReference/
+        //# API_GenerateDataKey.html) does not succeed, OnEncrypt MUST NOT modify
+        //# the encryption materials (structures.md#encryption-materials) and
+        //# MUST fail.
+        if maybeGenerateResponse.Failure? {
+          return Failure(maybeGenerateResponse.error);
+        }
+        var generateResponse := maybeGenerateResponse.value;
+
+        :- Need(generateResponse.IsWellFormed(), "Invalid response from KMS GenerateDataKey");
+        //= compliance/framework/aws-kms/aws-kms-mrk-aware-symmetric-keyring.txt#2.7
+        //# The Generate Data Key response's "KeyId" MUST be A valid AWS
+        //# KMS key ARN (aws-kms-key-arn.md#identifying-an-aws-kms-multi-region-
+        //# key).
+        :- Need(
+          ParseAwsKmsIdentifier(generateResponse.keyID).Success?,
+          "Invalid response from KMS GenerateDataKey:: Invalid Key Id"
+        );
+        :- Need(
+          materials.algorithmSuiteID.ValidPlaintextDataKey(generateResponse.plaintext),
+          "Invalid response from AWS KMS GenerateDataKey: Invalid data key"
+        );
+
+        var providerInfo :- UTF8.Encode(generateResponse.keyID);
+        :- Need(|providerInfo| < UINT16_LIMIT, "AWS KMS Key ID too long.");
+
+        var edk := Materials.EncryptedDataKey(
+          PROVIDER_ID,
+          providerInfo,
+          generateResponse.ciphertextBlob
+        );
+        var plaintextDataKey := generateResponse.plaintext;
+
+        var result := materials.WithKeys(Some(plaintextDataKey), [edk]);
+        return Success(result);
+      } else {
+        var encryptRequest := KMSUtils.EncryptRequest(
+          materials.encryptionContext,
+          grantTokens,
+          this.awsKmsKey,
+          materials.plaintextDataKey.value
+        );
+        var maybeEncryptResponse := KMSUtils.Encrypt(this.client, encryptRequest);
+
+        //= compliance/framework/aws-kms/aws-kms-mrk-aware-symmetric-keyring.txt#2.7
+        //= type=implication
+        //# If the call to AWS KMS Encrypt
+        //# (https://docs.aws.amazon.com/kms/latest/APIReference/
+        //# API_Encrypt.html) does not succeed, OnEncrypt MUST fail.
+        if maybeEncryptResponse.Failure? {
+          return Failure(maybeEncryptResponse.error);
+        }
+
+        var encryptResponse := maybeEncryptResponse.value;
+        :- Need(encryptResponse.IsWellFormed(), "Invalid response from KMS Encrypt");
+        //= compliance/framework/aws-kms/aws-kms-mrk-aware-symmetric-keyring.txt#2.7
+        //# If the Encrypt call succeeds The response's "KeyId" MUST be A valid
+        //# AWS KMS key ARN (aws-kms-key-arn.md#identifying-an-aws-kms-multi-
+        //# region-key).
+        :- Need(
+          ParseAwsKmsIdentifier(encryptResponse.keyID).Success?,
+          "Invalid response from AWS KMS Encrypt:: Invalid Key Id"
+        );
+
+        var providerInfo :- UTF8.Encode(encryptResponse.keyID);
+        :- Need(|providerInfo| < UINT16_LIMIT, "AWS KMS Key ID too long.");
+
+        var edk := Materials.EncryptedDataKey(
+          PROVIDER_ID,
+          providerInfo,
+          encryptResponse.ciphertextBlob
+        );
+
+        var result := materials.WithKeys(materials.plaintextDataKey, [edk]);
+        return Success(result);
+      }
+    }
+
+    //= compliance/framework/aws-kms/aws-kms-mrk-aware-symmetric-keyring.txt#2.8
+    //= type=implication
+    //# OnDecrypt MUST take decryption materials (structures.md#decryption-
+    //# materials) and a list of encrypted data keys
+    //# (structures.md#encrypted-data-key) as input.
+    method OnDecrypt(
+      materials: Materials.ValidDecryptionMaterials,
+      encryptedDataKeys: seq<Materials.EncryptedDataKey>
+    )
+      returns (res: Result<Materials.ValidDecryptionMaterials, string>)
+      requires Valid()
+      ensures Valid()
+      ensures OnDecryptPure(materials, res)
+      //= compliance/framework/aws-kms/aws-kms-mrk-aware-symmetric-keyring.txt#2.8
+      //= type=implication
+      //# If the decryption materials (structures.md#decryption-materials)
+      //# already contained a valid plaintext data key OnDecrypt MUST
+      //# immediately return the unmodified decryption materials
+      //# (structures.md#decryption-materials).
+      ensures
+        materials.plaintextDataKey.Some?
+      ==>
+        && res.Success?
+        && res.value == materials
+
+      ensures
+        && materials.plaintextDataKey.None?
+        && res.Success?
+      ==>
+        && res.value.plaintextDataKey.Some?
+        && exists edk | edk in encryptedDataKeys
+        ::
+          //= compliance/framework/aws-kms/aws-kms-mrk-aware-symmetric-keyring.txt#2.8
+          //= type=implication
+          //# *  Its provider ID MUST exactly match the value "aws-kms".
+          && edk.providerID == PROVIDER_ID
+          && DecryptCalled(
+            //= compliance/framework/aws-kms/aws-kms-mrk-aware-symmetric-keyring.txt#2.8
+            //= type=implication
+            //# To attempt to decrypt a particular encrypted data key
+            //# (structures.md#encrypted-data-key), OnDecrypt MUST call AWS KMS
+            //# Decrypt (https://docs.aws.amazon.com/kms/latest/APIReference/
+            //# API_Decrypt.html) with the configured AWS KMS client.
+            client,
+            //= compliance/framework/aws-kms/aws-kms-mrk-aware-symmetric-keyring.txt#2.8
+            //= type=implication
+            //# When calling AWS KMS Decrypt
+            //# (https://docs.aws.amazon.com/kms/latest/APIReference/
+            //# API_Decrypt.html), the keyring MUST call with a request constructed
+            //# as follows:
+            DecryptRequest(
+              awsKmsKey,
+              edk.ciphertext,
+              materials.encryptionContext,
+              grantTokens
+            ))
+          && DecryptResult(
+            //= compliance/framework/aws-kms/aws-kms-mrk-aware-symmetric-keyring.txt#2.8
+            //= type=implication
+            //# *  The "KeyId" field in the response MUST equal the configured AWS
+            //# KMS key identifier.
+            awsKmsKey,
+            //= compliance/framework/aws-kms/aws-kms-mrk-aware-symmetric-keyring.txt#2.8
+            //= type=implication
+            //# If the response does satisfies these requirements then OnDecrypt MUST
+            //# do the following with the response:
+            res.value.plaintextDataKey.value)
+          //= compliance/framework/aws-kms/aws-kms-mrk-aware-symmetric-keyring.txt#2.8
+          //= type=implication
+          //# *  The length of the response's "Plaintext" MUST equal the key
+          //# derivation input length (algorithm-suites.md#key-derivation-input-
+          //# length) specified by the algorithm suite (algorithm-suites.md)
+          //# included in the input decryption materials
+          //# (structures.md#decryption-materials).
+          && materials.algorithmSuiteID.ValidPlaintextDataKey(res.value.plaintextDataKey.value)
+
+    {
+
+      if (materials.plaintextDataKey.Some?) {
+        return Success(materials);
+      }
+
+      //= compliance/framework/aws-kms/aws-kms-mrk-aware-symmetric-keyring.txt#2.8
+      //# The set of encrypted data keys MUST first be filtered to match this
+      //# keyring's configuration.
+      var filter := new EncrypteDataKeyFilter(this.awsKmsArn);
+      var edksToAttempt :- Closures.FilterWithResult(encryptedDataKeys, filter);
+
+      //= compliance/framework/aws-kms/aws-kms-mrk-aware-symmetric-keyring.txt#2.8
+      //# For each encrypted data key in the filtered set, one at a time, the
+      //# OnDecrypt MUST attempt to decrypt the data key.
+      //# If this attempt
+      //# results in an error, then these errors MUST be collected.
+      var decryptClosure := new DecryptEncryptedDataKey(
+        materials,
+        this.client,
+        this.awsKmsKey,
+        this.grantTokens
+      );
+
+      //= compliance/framework/aws-kms/aws-kms-mrk-aware-symmetric-keyring.txt#2.8
+      //# If the response does not satisfies these requirements then an error
+      //# MUST be collected and the next encrypted data key in the filtered set
+      //# MUST be attempted.
+      var outcome := Closures.ReduceToSuccess(
+        edksToAttempt,
+        decryptClosure
+      );
+
+      return match outcome {
+        case Success(mat) =>
+          assert exists edk | edk in edksToAttempt
+          ::
+            && edk in encryptedDataKeys
+            && filter.Ensures(edk, Success(true))
+            && decryptClosure.Ensures(edk, Success(mat))
+            && DecryptCalled(
+              client,
+              DecryptRequest(
+                awsKmsKey,
+                edk.ciphertext,
+                materials.encryptionContext,
+                grantTokens
+              ))
+            && DecryptResult(awsKmsKey, mat.plaintextDataKey.value);
+          Success(mat)
+        //= compliance/framework/aws-kms/aws-kms-mrk-aware-symmetric-keyring.txt#2.8
+        //# If OnDecrypt fails to successfully decrypt any encrypted data key
+        //# (structures.md#encrypted-data-key), then it MUST yield an error that
+        //# includes all the collected errors.
+        case Failure(errors) =>
+          if |errors| == 0 then
+            Failure("Unable to decrypt data key: No Encrypted Data Keys found to match.")
+          else
+            var concatString := (s, a) => a + "\n" + s;
+            var error := Seq.FoldRight(
+              concatString,
+              errors,
+              "Unable to decrypt data key:\n"
+            );
+            Failure(error)
+      };
+    }
+  }
+
+  class EncrypteDataKeyFilter
+  extends ActionWithResult<Materials.EncryptedDataKey, bool, string>
+  {
+    const awsKmsKey: AwsKmsIdentifier
+
+    constructor(awsKmsKey: AwsKmsIdentifier) {
+      this.awsKmsKey := awsKmsKey;
+    }
+
+    predicate Ensures(
+      edk: Materials.EncryptedDataKey,
+      res: Result<bool, string>
+    ) {
+      && (
+          && res.Success?
+          && res.value
+        ==>
+          edk.providerID == PROVIDER_ID)
+    }
+
+    method Invoke(edk: Materials.EncryptedDataKey)
+      returns (res: Result<bool, string>)
+      ensures Ensures(edk, res)
+    {
+
+      if edk.providerID != PROVIDER_ID {
+        return Success(false);
+      }
+
+      if !UTF8.ValidUTF8Seq(edk.providerInfo) {
+        return Success(false);
+      }
+
+      var keyId :- UTF8.Decode(edk.providerInfo);
+      //= compliance/framework/aws-kms/aws-kms-mrk-aware-symmetric-keyring.txt#2.8
+      //# *  The provider info MUST be a valid AWS KMS ARN (aws-kms-key-
+      //# arn.md#a-valid-aws-kms-arn) with a resource type of "key" or
+      //# OnDecrypt MUST fail.
+      var arn :- ParseAwsKmsArn(keyId);
+
+      //= compliance/framework/aws-kms/aws-kms-mrk-aware-symmetric-keyring.txt#2.8
+      //# *  The the function AWS KMS MRK Match for Decrypt (aws-kms-mrk-match-
+      //# for-decrypt.md#implementation) called with the configured AWS KMS
+      //# key identifier and the provider info MUST return "true".
+      return Success(AwsKmsMrkMatchForDecrypt.AwsKmsMrkMatchForDecrypt(
+        this.awsKmsKey,
+        AwsKmsArnIdentifier(arn)
+      ));
+    }
+  }
+
+  class DecryptEncryptedDataKey
+  extends ActionWithResult<
+    Materials.EncryptedDataKey,
+    Materials.CompleteDecryptionMaterials,
+    string>
+  {
+    const materials: Materials.PendingDecryptionMaterials
+    const client: IAmazonKeyManagementService
+    const awsKmsKey: AwsKmsIdentifierString
+    const grantTokens: KMSUtils.GrantTokens
+
+    constructor(
+      materials: Materials.PendingDecryptionMaterials,
+      client: IAmazonKeyManagementService,
+      awsKmsKey: AwsKmsIdentifierString,
+      grantTokens: KMSUtils.GrantTokens
+    )
+      ensures 
+      && this.materials == materials
+      && this.client == client
+      && this.awsKmsKey == awsKmsKey
+      && this.grantTokens == grantTokens
+    {
+      this.materials := materials;
+      this.client := client;
+      this.awsKmsKey := awsKmsKey;
+      this.grantTokens := grantTokens;
+    }
+
+    predicate Ensures(
+      edk: Materials.EncryptedDataKey,
+      res: Result<Materials.CompleteDecryptionMaterials, string>
+    ) {
+        res.Success?
+      ==>
+        && res.value.Valid()
+        && OnDecryptPure(this.materials, res)
+        && DecryptCalled(
+          client,
+          DecryptRequest(
+            awsKmsKey,
+            edk.ciphertext,
+            materials.encryptionContext,
+            grantTokens
+          )
+        )
+        && DecryptResult(awsKmsKey, res.value.plaintextDataKey.value)
+    }
+
+    method Invoke(
+      edk: Materials.EncryptedDataKey
+    ) returns (res: Result<Materials.CompleteDecryptionMaterials, string>)
+      ensures Ensures(edk, res)
+    {
+
+      var decryptRequest := KMSUtils.DecryptRequest(
+        awsKmsKey,
+        edk.ciphertext,
+        materials.encryptionContext,
+        grantTokens
+      );
+
+      var decryptResponse :- KMSUtils.Decrypt(this.client, decryptRequest);
+
+      :- Need(
+        && decryptResponse.keyID == this.awsKmsKey
+        && this.materials.algorithmSuiteID.ValidPlaintextDataKey(decryptResponse.plaintext)
+        , "Invalid response from KMS Decrypt");
+
+      var result := this.materials.WithPlaintextDataKey(decryptResponse.plaintext);
+      return Success(result);
+    }
+  }
+}
